theories/L3_flattenedApp/wcbvEval.v
@@ -53,16 +53,18 @@ Inductive WcbvEval (p:environ Term) : Term -> Term -> Prop :=
               WcbvEval p (TApp fn arg) (TApp efn arg1)
 | wCase: forall mch i n ml args args' brs cs s,
            WcbvEval p mch (TConstruct i n args) ->
-           i = (fst (fst ml)) ->
-           tskipn (snd (fst ml)) args = Some args' ->  (* drop parameters *)
+           i = fst ml ->
+           tskipn (snd ml) args = Some args' ->  (* drop parameters *)
            whCaseStep n args' brs = Some cs ->
            WcbvEval p cs s ->
            WcbvEval p (TCase ml mch brs) s
-| wCaseCong: forall ml mch emch brs ebrs,
+| wCaseCong: forall ml mch emch brs,
            WcbvEval p mch emch ->
            ~ isConstruct emch ->
+           (*************
            WcbvEvals p brs ebrs ->
-           WcbvEval p (TCase ml mch brs) (TCase ml emch ebrs)
+*********************)
+           WcbvEval p (TCase ml mch brs) (TCase ml emch brs)
 | wWrong: WcbvEval p TWrong TWrong
 with WcbvEvals (p:environ Term) : Terms -> Terms -> Prop :=
 | wNil: WcbvEvals p tnil tnil
@@ -347,8 +349,8 @@ Function wcbvEval
         | TCase ml mch brs =>
           match wcbvEval n mch with
             | Ret (TConstruct i r args) =>
-              if eq_dec i (fst (fst ml)) then
-                match tskipn (snd (fst ml)) args with
+              if eq_dec i (fst ml) then
+                match tskipn (snd ml) args with
                   | None => raise "wcbvEval: Case, tskipn"
                   | Some ts => match whCaseStep r ts brs with
                                  | None => raise "wcbvEval: Case, whCaseStep"
@@ -356,11 +358,7 @@ Function wcbvEval
                                end
                 end
               else raise "wcbvEval: TCase: i doesn't match"
-            | Ret emch =>
-              match wcbvEvals n brs with
-                | Exc s => raise s
-                | Ret ebrs => Ret (TCase ml emch ebrs)
-              end
+            | Ret emch => Ret (TCase ml emch brs)
             | Exc s => Exc s
           end
         | TLetIn nm df bod =>
@@ -426,7 +424,7 @@ Proof.
     try (solve[not_isApp]).
   - subst. specialize (H _ e1). specialize (H0 _ p1). 
     refine (wCase _ _ _ _ _ _ _); eassumption || reflexivity.
-  - specialize (H _ e1). specialize (H0 _ e2). 
+  - specialize (H _ e1). 
     eapply wCaseCong; try assumption. 
     destruct emch; try not_isConstruct. contradiction. 
   - eapply wLetIn.
@@ -437,7 +435,7 @@ Qed.
 (* need this strengthening to large-enough fuel to make the induction
 ** go through
 *)
-Lemma WcbvEval_wcbvEval:
+Lemma pre_WcbvEval_wcbvEval:
     (forall t s, WcbvEval p t s ->
         exists n, forall m, m >= n -> wcbvEval (S m) t = Ret s) /\
     (forall ts ss, WcbvEvals p ts ss ->
@@ -487,12 +485,11 @@ Proof.
     assert (l1:= max_fst x x0). assert (l2:= max_snd x x0).
     rewrite (j m (max x x0)); try omega.
     rewrite hx; try omega. rewrite e0; try omega. rewrite e1; try omega.
-    destruct (inductive_dec i (fst (fst ml))).
+    destruct (inductive_dec i (fst ml)).
     + apply hx0; try omega.
     + elim n0; assumption.
-  - destruct H; destruct H0. exists (S (max x x0)). intros m h.
-    assert (l:= max_fst x x0). assert (l2:= max_snd x x0). cbn.
-    rewrite (j m (max x x0)); try omega. rewrite H; try omega.
+  - destruct H. exists (S x). intros m h. cbn.
+    rewrite (j m x); try omega. rewrite (H (m - 1)); try omega.
     destruct emch; try rewrite H0; try reflexivity; try omega.
     elim n. auto.
   - destruct H; destruct H0. exists (S (max x x0)). intros m h.
@@ -501,582 +498,29 @@ Proof.
     rewrite H0. reflexivity. omega.
 Qed.
 
+Lemma WcbvEval_wcbvEval:
+  forall t s, WcbvEval p t s ->
+             exists n, forall m, m >= n -> wcbvEval m t = Ret s.
+Proof.
+  intros t s h.
+  destruct (proj1 pre_WcbvEval_wcbvEval _ _ h).
+  exists (S x). intros m hm. specialize (H (m - 1)).
+  assert (k: m = S (m - 1)). { omega. }
+  rewrite k. apply H. omega.
+Qed.
+
+Lemma WcbvEval_single_valued:
+  forall t s, WcbvEval p t s -> forall u, WcbvEval p t u -> s = u.
+Proof.
+  intros t s h0 u h1.
+  assert (j0:= WcbvEval_wcbvEval h0).
+  assert (j1:= WcbvEval_wcbvEval h1).
+  destruct j0 as [x0 k0].
+  destruct j1 as [x1 k1].
+  specialize (k0 (max x0 x1) (max_fst x0 x1)).
+  specialize (k1 (max x0 x1) (max_snd x0 x1)).
+  rewrite k0 in k1. injection k1. intuition.
+Qed.
+
 End wcbvEval_sec.
 
-
-(**** scratch below here ****
-(** wcbvEval is monotonic in fuel **)
-Goal
-  (forall t n p,  wcbvEval n t <> TUnknown"" ->
-                   wcbvEval n t = wcbvEval (S n) p t).
-induction t; intros. 
-- destruct n0; simpl in H; intuition.
-- destruct n; simpl in H. intuition. reflexivity.
-- destruct n. simpl in H. intuition.  simpl in H. simpl.
-  change (TCast (wcbvEval n t1) c t2 = TCast (wcbvEval (S n) p t1) c t2).
-  rewrite IHt1. reflexivity. intros h. rewrite <- h in H.
-
-unfold wcbvEval in H. simpl.
-
-
-         (forall (t s:Term), wcbvEval p t s ->
-             exists n, s = wcbvEval n t) /\
-         (forall ts ss, WcbvEvals p ts ss ->
-             exists n, ss = tmap (wcbvEval n p) ts).
-Goal
-  forall (p:environ Term),
-         (forall (t s:Term), wcbvEval p t s ->
-             exists n, s = wcbvEval n t) /\
-         (forall ts ss, WcbvEvals p ts ss ->
-             exists n, ss = tmap (wcbvEval n p) ts).
-
-(** WcbvEval and wcbvEval are the same relation **)
-Goal
-  forall (p:environ Term),
-         (forall (t s:Term), WcbvEval p t s ->
-             exists n, s = wcbvEval n t) /\
-         (forall ts ss, WcbvEvals p ts ss ->
-             exists n, ss = tmap (wcbvEval n p) ts).
-intros p.
-apply WcbvEvalEvals_ind; intros; try (exists 1; reflexivity).
-- destruct H. exists (S x). subst.
-  assert (j:= proj2 (lookupDfn_LookupDfn _ _ _) l).
-  simpl. rewrite j. reflexivity.
-- destruct H. destruct H0. destruct H1.
-  exists (S (x + x0 + x1)). subst. unfold whBetaStep. simpl.
-
-
-
-
-
-
-Qed.
-
-(** use a timer to make this Terminate **)
-Fixpoint wcbvEval (tmr:nat) (p:environ Term) (t:Term) {struct tmr} : nat * Term :=
-  match tmr with 
-    | 0 => (0, TUnknown "time")          (** out of time  **)
-    | S n => match t with  (** look for a redex **)
-               | TConst nm => match (lookupDfn nm p) with
-                                | Some t => wcbvEval n t
-                                | None =>  (0, TUnknown nm)
-                              end
-               | TApp fn a1 args =>
-                 let (_,efn) := wcbvEval n fn in
-                 match efn with
-                   | TLambda _ _ bod =>
-                     let (_,wharg) := wcbvEval n a1 in
-                     wcbvEval n (whBetaStep bod wharg args)
-                   | TFix dts m =>
-                     wcbvEval n (whFixStep dts m (tcons a1 args))
-                   | TConstruct _ r =>
-                     let (_,ea1) := wcbvEval n a1 in
-                     let eargs := 
-                         tmap (fun t =>
-                                 let (_,et) := wcbvEval n t in et) args in
-                     (n, TApp efn ea1 eargs)
-                   | _ => (n, TUnknown"App")
-                 end
-               | TCase np _ mch brs =>
-                 let (_,emch) := wcbvEval n mch in
-                 match emch with 
-                   | TConstruct _ r => wcbvEval n (whCaseStep r tnil brs)
-                   | TApp (TConstruct _ r) arg args =>
-                     wcbvEval n p
-                              (whCaseStep r (tskipn np (tcons arg args)) brs)
-                   | _ => (n, TUnknown"Case")
-                 end
-               | TLetIn nm df ty bod =>
-                 let (_,df') := wcbvEval n df in
-                 wcbvEval n (instantiate df' 0 bod)
-               | TCast t1 ck t2 => (n, TCast (snd (wcbvEval n t1)) ck t2)
-               (** already in whnf ***)
-               | TLambda nn ty t => (n, TLambda nn ty t)
-               | TProd nn ty t => (n, TProd nn ty t)
-               | TFix mfp br => (n, TFix mfp br)
-               | TConstruct i cn => (n, TConstruct i cn)
-               | TInd i => (n, TInd i)
-               | TSort srt => (n, TSort srt)
-               (** should never appear **)
-               | TRel _ => (0, TUnknown "TRel")
-               | TUnknown s => (0, TUnknown s)
-             end
-  end.
-
-(** If wcbvEval has fuel left, then it has reached a weak normal form **)
-(**
-Goal
-  forall (p:environ Term) t s n m, (wcbvEval n t) = (S m, s) -> WNorm s.
-***)
-
-(** WcbvEval and wcbvEval are the same relation **)
-Goal
-  forall (p:environ Term),
-         (forall (t s:Term), WcbvEval p t s ->
-             exists n, s = snd (wcbvEval n t)) /\
-         (forall ts ss, WcbvEvals p ts ss ->
-        exists n, ss = tmap (fun t => let (_,et) := wcbvEval n t in et) ts).
-intros p.
-apply WcbvEvalEvals_ind; intros; try (exists 1; reflexivity).
-- destruct H. exists (S x). subst.
-  assert (j:= proj2 (lookupDfn_LookupDfn _ _ _) l).
-  simpl. rewrite j. reflexivity.
-- destruct H. destruct H0. destruct H1.
-  exists (S (x + x0 + x1)). simpl.
-
-
-
-
-(***** scratch below here ****************
-
-
-Goal forall (p:environ Term) t s, WcbvEval p t s -> crct p t -> wNorm s = true.
-induction 1; destruct 1. 
-- apply IHWcbvEval. split. assumption. unfold weaklyClosed. intros nmx j.
-  unfold weaklyClosed in H2. apply H2. inversion H1. subst.
-  + specialize (H2 nm). unfold poccTrm in H2; simpl in H2.
-    rewrite string_eq_bool_rfl in H2. intuition.
-  + apply sBeta.
-
-
-
-HERE
-
-  + destruct (string_dec nmx nm).
-    * subst. unfold poccTrm. rewrite string_eq_bool_rfl. reflexivity.
-    * inversion H1. subst. inversion_clear H0. inversion H.
-  
-    simpl in H3.
-
-  + unfold poccTrm. inversion H1. subst. inversion h. unfold weaklyClosed in H3.
-    simpl in H3.
-
-
-
-
-Goal forall (p:environ Term), 
-  (forall t s, WcbvEval p t s -> crct p t -> wNorm s = true) /\
-  (forall ts ss, WcbvEvals p ts ss ->
-        Forall (crct p) ts -> Forall (fun s => wNorm s = true) ss).
-intros p.
-apply WcbvEvalEvals_ind.
-- intros nm t s q h1 h2 h3 h4. apply h3. inversion h2; subst.
-  + split.
-    * inversion h4. auto.
-    * unfold  weaklyClosed. intros nm1 j1.
-      simpl in j1. assert (j2:= string_eq_bool_eq _ _ j1). subst.
-      assert (j3:= proj2 (lookupDFN_LookupDFN _ _ _) H).
-      unfold lookupDfn. rewrite j3. intros j4. discriminate.
-  + destruct h4. split. auto. unfold weaklyClosed.
-    intros nm1 h4. simpl in h4.
-
-induction 1; inversion 1.
-- subst. elim (ncrct_nil_TConst nm _ _ H1); reflexivity.
-- subst. apply IHWcbvEval.
-
-HERE
-
-
-
-
-(***
-Lemma instantiate_arg_resp_WcbvEval:
-  (forall p ia2 s, WcbvEval p ia2 s -> 
-    forall a1 a2 bod, ia2 = (instantiate 0 bod a2) -> 
-    WcbvEval p a1 a2 -> WcbvEval p (instantiate 0 bod a1) s) /\
-  (forall p ia2 s, WcbvEvals p ia2s ss -> 
-    forall a1 a2 bod, ia2 = (instantiate 0 bod a2) -> 
-    WcbvEval p a1 a2 -> WcbvEval p (instantiate 0 bod a1) s)
-induction 1. intros ax a2 bod heq h.
-- eapply IHWcbvEval. intuition. assumption.
-- eapply IHWcbvEval3. assumption.
-- eapply IHWcbvEval2. assumption.
-- eapply 
-***)
-
-Lemma nat_compare_Gt: forall n, nat_compare (S n) n = Gt.
-induction n; intuition.
-Qed.
-Lemma nat_compare_Lt: forall n, nat_compare n (S n) = Lt.
-induction n; intuition.
-Qed.
-Lemma nat_compare_Eq: forall n, nat_compare n n = Eq.
-induction n; intuition.
-Qed.
-
-Lemma instantiate_is_Const:
-  forall m bod a nm, instantiate m bod a = TConst nm ->
-                        a = TConst nm \/ bod = TConst nm.
-induction bod; intros a nm h; simpl in h; try discriminate h.
-- case_eq (nat_compare m n); intro j; rewrite j in h;
-  try assumption; try discriminate h. intuition.
-- intuition.
-Qed.
-
-(**
-Goal
-  forall p ia2 s, WcbvEval p ia2 s -> 
-     forall bod a1 a2, ia2 = (instantiate 0 bod a2) -> WcbvEval p a1 a2 ->
-                    WcbvEval p (instantiate 0 bod a1) s.
-induction 1; intros bodx ax a2 heq h.
-- symmetry in heq. case (instantiate_is_Const _ _ _ _ heq); intro j.
-
-Lemma WcbvEval_unique:
-  forall (p:environ Term) (t s1:Term),
-    WcbvEval p t s1 -> forall (s2:Term), WcbvEval p t s2 -> s1 = s2.
-induction 1.
-- inversion_clear 1. eapply IHWcbvEval.
-  assert (j: t = t0). rewrite H in H2; injection H2; intuition.
-  rewrite j; assumption.
-- inversion_clear 1.
-  + eapply IHWcbvEval3. unfold whBetaStep. unfold whBetaStep in H5.
-    injection (IHWcbvEval1 _ H3); intros; subst.
-***)
-
-
-
-(**
-Ltac Tran_step := eapply Relation_Operators.rt1n_trans.
-
-Ltac const_step :=
-  tran_step; [eapply sConst; unfold lookupDfn, lookupDFN; simpl; reflexivity|].
-**)
-(***
-Goal
-  forall p fn nm ty bod a1 a1' s args,
-    clos_trans_n1 Term (wndEval p) fn (TLambda nm ty bod) ->
-    clos_trans_n1 Term (wndEval p) a1 a1' ->
-    clos_trans_n1 Term (wndEval p) (whBetaStep nm bod a1' args) s ->
-    clos_trans_n1 Term (wndEval p) (TApp fn (a1 :: args)) s.
-intros p fn nm ty bod a1 a1' s args hfn ha1 hstep.
-inversion hfn; inversion ha1; inversion hstep.
-- tran_step. eassumption.
-  tran_step. eapply sAppArgs. eapply saHd. eassumption.    
-  tran_step. eapply sBeta. eassumption.
-- tran_step. eapply sAppFun. eassumption.
-  tran_step. eapply sAppArgs. eapply saHd. eassumption.
-  tran_step. eapply sBeta. eassumption.
-- tran_step. eapply sAppFun. eassumption.
-  tran_step. eapply sAppArgs. eapply saHd. eapply tn1_step. eassumption.
-  tran_step. eapply sBeta. eassumption.
-***)
-
-
-(**
-Goal
-  forall p a a',
-    clos_refl_trans Term (wndEval p) a a' ->
-    forall bod args,
-      clos_refl_trans Term (wndEval p) (mkApp (instantiate 0 bod a) args)
-                         (mkApp (instantiate 0 bod a') args).
-intros p a a' h bod. induction h; intro args.
-- apply rt_step.
- Check  Relation_Operators.rt1n_trans.
-
-
-
-Goal
-  forall p fn nm ty bod a1 a1' s args,
-    clos_refl_trans_1n Term (wndEval p) fn (TLambda nm ty bod) ->
-    clos_refl_trans_1n Term (wndEval p) a1 a1' ->
-    clos_refl_trans_1n Term (wndEval p) (whBetaStep nm bod a1' args) s ->
-    clos_refl_trans_1n Term (wndEval p) (TApp fn (a1 :: args)) s.
-intros p fn nm ty bod a1 a1' s args hfn ha1 hstep.
-inversion hfn; inversion ha1; inversion hstep.
-- tran_step. subst. eapply sBeta. subst. auto. 
-- tran_step. subst. eapply sBeta. subst. eassumption.
-- assert (j: clos_refl_trans_1n Term (wndEval p) a1 a1').
-  tran_step; eassumption.
-  tran_step. eapply sBeta. rewrite H3. destruct nm.
-  + simpl. simpl in H3. rewrite H3. eapply rt1n_refl.
-  + simpl. simpl in H3. rewrite <- H3.
--
-
-
- tran_step. eapply sAppArgs. eapply saHd. eassumption.
-  tran_step.
-
-  eapply (t1n_trans _ (wndEval p)). eapply t1n_step. eapply sAppArgs. eapply saHd.
-  eapply clos_t1n_trans. 
-
-eapply (t1n_trans _ (wndEval p)).
-
-
- Check (t1n_trans _ _ _ H1).
-  tran_step. eapply sAppArgs. eapply saHd. eassumption.
-  tran_step. eapply sBeta. eassumption.
-- tran_step. eapply sAppFun. eassumption.
-
-
-Goal
-  forall p fn nm ty bod a1 a1' s args,
-    clos_trans_1n Term (wndEval p) fn (TLambda nm ty bod) ->
-    clos_trans_1n Term (wndEval p) a1 a1' ->
-    clos_trans_1n Term (wndEval p) (whBetaStep nm bod a1' args) s ->
-    clos_trans_1n Term (wndEval p) (TApp fn (a1 :: args)) s.
-intros p fn nm ty bod a1 a1' s args hfn ha1 hstep.
-inversion hfn; inversion ha1; inversion hstep.
-- tran_step. eapply sAppFun. eassumption.
-  tran_step. eapply sAppArgs. eapply saHd. eassumption.    
-  tran_step. eapply sBeta. eassumption.
-- tran_step. eapply sAppFun. eassumption.
-  tran_step. eapply sAppArgs. eapply saHd. eassumption.
-  tran_step. eapply sBeta. eassumption.
-- tran_step. eapply sAppFun. eassumption.
-
-  tran_step. eapply sAppArgs. eapply saHd. eassumption.
-  tran_step. eapply sBeta. eassumption.
-
-
-Goal
-  forall p fn nm ty bod a1 a1' s args,
-    clos_trans Term (wndEval p) fn (TLambda nm ty bod) ->
-    clos_trans Term (wndEval p) a1 a1' ->
-    clos_trans Term (wndEval p) (whBetaStep nm bod a1' args) s ->
-    clos_trans Term (wndEval p) (TApp fn (a1 :: args)) s.
-intros p fn nm ty bod a1 a1' s args hfn ha1 hstep.
-inversion hfn; inversion ha1; inversion hstep.
-- tran_step. eapply sAppFun. eassumption.
-  tran_step. eapply sAppArgs. eapply saHd. eassumption.    
-  tran_step. eapply sBeta.
-  eassumption.
-unfold whBetaStep in H3.
-***)
-
-(**
-Ltac Tran_step := eapply Relation_Operators.rt1n_trans.
-
-Goal forall p t t', WcbvEval p t t' -> clos_refl_trans_1n _ (wndEval p) t t'.
-induction 1.
-- Tran_step. eapply sConst. rewrite H. reflexivity. assumption.
-- tran_step. eapply sAppFun.
-Check (rt_refl Term (wndEval p)). _ (wndEval p) _ IHWcbvEval1).
-**)
-
-Definition Nat := nat.
-Definition typedef := ((fun (A:Type) (a:A) => a) Nat 1).
-Quote Definition q_typedef := Eval compute in typedef.
-Quote Recursively Definition p_typedef := typedef.
-Definition P_typedef := program_Program p_typedef nil.
-Definition Q_typedef := 
-  Eval compute in (wcbvEval 100 (env P_typedef) (main P_typedef)).
-Goal snd Q_typedef = q_typedef.
-reflexivity.
-Qed.
-
-
-Definition II := fun (A:Type) (a:A) => a.
-Quote Definition q_II := Eval compute in II.
-Quote Recursively Definition p_II := II.
-Definition P_II := program_Program p_II nil.
-Definition Q_II :=
-  Eval compute in (wcbvEval 4 (env P_II)) (main P_II).
-Goal snd Q_II = q_II.
-reflexivity.
-Qed.
-
-(***
-Eval cbv in (wcbvEval 4 p_II) (main p_II).
-Quote Recursively Definition II_nat_pgm := (II nat).
-Print II_nat_pgm.
-Eval compute in (wcbvEval 4 II_nat_pgm) (main II_nat_pgm).
-
-
-Quote Definition II_2_Term := (II nat 2).
-Print II_2_Term.
-Eval compute in II_2_Term.
-Quote Recursively Definition II_2_program := (II nat 2).
-Print II_2_program.
-Quote Definition two_Term := 2.
-
-Eval cbv in (wcbvEval 4 II_2_program) (main II_2_program).
-
-Quote Recursively Definition p_plus22 := (plus 2 2).
-Print p_plus22.
-Quote Definition q_ans := 4.
-Eval cbv in (wcbvEval 20 p_plus22) (main p_plus22).
-
-Eval compute in (plus 1 2).
-Quote Recursively Definition p_plus12 := (plus 1 2).
-Eval cbv in (wcbvEval 99 p_plus12) (main p_plus12).
-
-Quote Recursively Definition p_anon := ((fun (_:nat) => 1 + 3) (3 * 3)).
-Eval cbv in (wcbvEval 20 p_anon) (main p_anon).
-
-Fixpoint even (n:nat) : bool :=
-  match n with
-    | 0 => true
-    | (S n) => odd n
-  end
-with
-odd (n:nat) : bool :=
-  match n with
-    | 0 => false
-    | (S n) => even n
-  end.
-
-Quote Recursively Definition p_even99 := (even 99).
-Time Eval cbv in (wcbvEval 500 p_even99) (main p_even99).
-Quote Recursively Definition p_odd99 := (odd 99).
-Time Eval cbv in (wcbvEval 500 p_odd99) (main p_odd99).
-
-
-Fixpoint slowFib (n:nat) : nat :=
-  match n with
-    | 0 => 0
-    | S m => match m with
-               | 0 => 1
-               | S p => slowFib p + slowFib m
-             end
-  end.
-Eval compute in (slowFib 0).
-Eval compute in (slowFib 1).
-Eval compute in (slowFib 2).
-Eval compute in (slowFib 3).
-Eval compute in (slowFib 4).
-Quote Recursively Definition p_slowFib1 := (slowFib 1).
-Quote Recursively Definition p_slowFib2 := (slowFib 2).
-Quote Recursively Definition p_slowFib3 := (slowFib 3).
-Quote Recursively Definition p_slowFib4 := (slowFib 4).
-Quote Recursively Definition p_slowFib5 := (slowFib 5).
-Quote Recursively Definition p_slowFib6 := (slowFib 6).
-Quote Recursively Definition p_slowFib7 := (slowFib 7).
-Quote Recursively Definition p_slowFib10 := (slowFib 10).
-Quote Recursively Definition p_slowFib15 := (slowFib 15).
-Eval cbv in (wcbvEval 99 p_slowFib3) (main p_slowFib3).
-Eval cbv in (wcbvEval 99 p_slowFib4) (main p_slowFib4).
-Eval cbv in (wcbvEval 99 p_slowFib5) (main p_slowFib5).
-Eval cbv in (wcbvEval 99 p_slowFib6) (main p_slowFib6).
-Time Eval cbv in (wcbvEval 99 p_slowFib7) (main p_slowFib7).
-Time Eval cbv in (wcbvEval 99 p_slowFib10) (main p_slowFib10).
-Time Eval cbv in (wcbvEval 200 p_slowFib15) (main p_slowFib15).
-
-
-Fixpoint fibrec (n:nat) (fs:nat * nat) {struct n} : nat :=
-  match n with
-    | 0 => fst fs
-    | (S n) => fibrec n (pair ((fst fs) + (snd fs)) (fst fs))
-  end.
-Definition fib : nat -> nat := fun n => fibrec n (pair 0 1).
-
-Eval compute in (fib 0).
-Eval compute in (fib 1).
-Eval compute in (fib 2).
-Eval compute in (fib 3).
-Eval compute in (fib 4).
-Eval compute in (fib 6).
-Quote Recursively Definition p_fib1 := (fib 1).
-Quote Recursively Definition p_fib2 := (fib 2).
-Quote Recursively Definition p_fib3 := (fib 3).
-Quote Recursively Definition p_fib4 := (fib 4).
-Quote Recursively Definition p_fib5 := (fib 5).
-Quote Recursively Definition p_fib6 := (fib 6).
-Quote Recursively Definition p_fib7 := (fib 7).
-Quote Recursively Definition p_fib10 := (fib 10).
-Quote Recursively Definition p_fib15 := (fib 15).
-Eval cbv in (wcbvEval 20 p_fib1) (main p_fib1).
-Eval cbv in (wcbvEval 30 p_fib2) (main p_fib2).
-Eval cbv in (wcbvEval 40 p_fib3) (main p_fib3).
-Eval cbv in (wcbvEval 50 p_fib4) (main p_fib4).
-Eval cbv in (wcbvEval 60 p_fib5) (main p_fib5).
-Eval cbv in (wcbvEval 60 p_fib6) (main p_fib6).
-Time Eval cbv in (wcbvEval 70 p_fib7) (main p_fib7).
-Time Eval cbv in (wcbvEval 70 p_fib10) (main p_fib10).
-Time Eval cbv in (wcbvEval 200 p_fib15) (main p_fib15).
-
-
-Quote Recursively Definition l_fib4 := (let x := 4 in fib x).
-Eval cbv in (wcbvEval 50 l_fib4) (main l_fib4).
-
-Fixpoint evenP (n:nat) {struct n} : bool :=
-  match n with
-    | 0 => true
-    | S p => (oddP p)
-  end
-with oddP (n:nat) : bool :=
-  match n with
-    | 0 => false
-    | S p => evenP p
-  end.
-
-Quote Recursively Definition p_evenOdd := (even 100).
-Quote Recursively Definition f_evenOdd := (odd 100).
-Eval cbv in (wcbvEval 500 p_evenOdd) (main p_evenOdd).
-Eval cbv in (wcbvEval 500 f_evenOdd) (main f_evenOdd).
-
-Quote Recursively Definition l_evenOdd := (even (let x := 50 in 2 * x)).
-Time Eval cbv in (wcbvEval 500 l_evenOdd) (main l_evenOdd).
-Time Eval cbv in (wcbvEval 5000 l_evenOdd) (main l_evenOdd).
-
-Parameter axiom:nat.
-Quote Recursively Definition p_axiom := (let x := axiom in 2 * x).
-Print p_axiom.
-Time Eval cbv in (wcbvEval 100 p_axiom) (main p_axiom).
-Time Eval cbv in (wcbvEval 200 p_axiom) (main p_axiom).
-
-***********)
-
-(***
-Goal forall p s t,
-       WcbvEval p s t -> exists (n m:nat), wcbvEval n s  = (S m, t).
-induction 1.
-- destruct IHWcbvEval. destruct H1. exists (S x). exists x0.
-  simpl. rewrite H. assumption.
-- destruct IHWcbvEval1, IHWcbvEval2, IHWcbvEval3.
-  destruct H2, H3, H4.
-  exists (S (x + x0 + x1)). exists (S (x2 + x3 + x4)).
-  simpl.
-***)
-
-(* Coq doesn't evaluate the type of a cast *)
-Eval cbv in  3 : ((fun n:Type => nat) Prop).
-Eval lazy in  3 : ((fun n:Type => nat) Prop).
-Eval hnf in  3 : ((fun n:Type => nat) Prop).
-Eval vm_compute in  3 : ((fun n:Type => nat) Prop).
-
-Goal 
-  forall (t s:Term) (n m:nat) (e:environ Term),
-  wcbvEval (S n) e t = (S m,s) -> wNorm s = true.
-intros t; induction t; intros; try discriminate;
-try (injection H; intros h1 h2; rewrite <- h1; auto; subst).
-- simpl. simpl in H. rewrite h2 in H. rewrite h1. erewrite IHt1.
-
-
-Lemma not_ltb_n_0: forall (n:nat), ltb n 0 = false.
-induction n; unfold ltb; reflexivity.
-Qed.
-
-Lemma wcbvEval_up:
-  forall (n:nat) (p:program) (s:Term),
-   closedTerm 0 s = true -> fst (wcbvEval n s) > 0 ->
-   snd (wcbvEval n s) = snd (wcbvEval (S n) p s).
-intros n p s h1. induction n. simpl. omega.
-intros h2.
-induction s; simpl in h1; try rewrite not_ltb_n_0 in h1;
-try discriminate; try reflexivity.
-Admitted.
-
-(***
-intros n p s h. induction n. simpl. intro h1. omega.
-intro h1. induction s; try reflexivity.
-- rewrite IHs2.
-***)
-
-Goal forall (strt:nat) (p:program) (s:Term),
-       wNorm s = true -> snd (wcbvEval strt p s) = s.
-intros strt p s h. induction strt. reflexivity.
-induction s; simpl in h; try discriminate h; try reflexivity.
-- rewrite <- IHstrt. rewrite -> IHstrt at 1. rewrite <- wcbvEval_up. reflexivity. simpl.
-
-- rewrite <- IHstrt. rewrite -> IHstrt at 1. admit.
-- rewrite <- IHstrt. rewrite -> IHstrt at 1. admit.
-- rewrite <- IHstrt. rewrite -> IHstrt at 1. admit.
-- rewrite <- IHstrt. rewrite -> IHstrt at 1. admit.
-Qed.
-
-Goal forall (strt:nat) (p:program) (s:Term),
-       fst (wcbvEval strt p s) > 0 -> wNorm (snd (wcbvEval strt p s)) = true.
-intros strt p s h. induction s; unfold wcbvEval; simpl.
-
-*******************)
-*****)
