theories/L2_5_box/L2_5.v
@@ -2,3 +2,4 @@
 
 Require Export L2_5.compile.
 Require Export L2_5.term L2_5.program L2_5.wndEval L2_5.wcbvEval L2_5.wNorm.
+Require Export L2_5.stripEvalCommute.
